TestModels/Composite/dafny/PrimaryProject/Model/primary-project.smithy
@@ -1,8 +1,6 @@
 namespace simple.composite.primaryproject
 
-use simple.composite.dependencyproject#DependencyService
-use simple.composite.dependencyproject#IdentityOperationInput
-use simple.composite.dependencyproject#IdentityOperationOutput
+use simple.composite.dependencyproject#SomeDependencyOperation
 
 @aws.polymorph#localService(
   sdkId: "PrimaryProject",
@@ -10,18 +8,17 @@ use simple.composite.dependencyproject#IdentityOperationOutput
 ) service PrimaryProject {
   version: "2021-11-01",
   resources: [],
-  operations: [ IdentityOperation, IdentityOperationOnDependency ],
+  operations: [ SomePrimaryOperation, SomeDependencyOperation ],
   errors: [],
 }
 
 structure PrimaryProjectConfig {}
 
-operation IdentityOperation {
-  input: IdentityOperationInput,
-  output: IdentityOperationOutput,
+operation SomePrimaryOperation {
+  input: SomePrimaryOperationInput,
+  output: SomePrimaryOperationOutput,
 }
 
-operation IdentityOperationOnDependency {
-  input: IdentityOperationInput,
-  output: IdentityOperationOutput,
-}
+structure SomePrimaryOperationInput {}
+
+structure SomePrimaryOperationOutput {}
